src/PredCalc/NAryEquivLemmas.v
@@ -28,7 +28,6 @@ Notation "(⇔)ₗ" := FIff (only parsing) : refiney_scope.
 Notation "( X ⇔.)ₗ" := (FIff X) (only parsing) : refiney_scope.
 Notation "(.⇔ X )ₗ" := (λ Y, FIff X Y) (only parsing) : refiney_scope.
 
-
 Section n_ary_lemmas.
   Context {M : model}.
 
@@ -46,9 +45,8 @@ Section n_ary_lemmas.
   Implicit Types Bs Cs Ds : list formula.
   Implicit Types vs : list value.
 
-
   Lemma f_eqlist_nil :
-    <! ⌜[] =* []⌝ !> ≡ₗ@{M} <! true !>.
+    <! ⌜[] =* []⌝ !> ≡@{formula} <! true !>.
   Proof. unfold FEqList. reflexivity. Qed.
 
   Lemma f_eqlist_cons t1 t2 ts1 ts2
@@ -638,7 +636,7 @@ Section n_ary_lemmas.
   Lemma f_existslist_one_point xs ts A `{OfSameLength _ _ xs ts} :
     NoDup xs →
     (list_to_set xs) ∩ ⋃ (term_fvars <$> ts) = ∅ →
-    <! ∃* xs, ⌜$(TVar <$> xs) =* ts⌝ ∧ A !> ≡ <! A[; *xs \ *ts ;] !>.
+    <! ∃* xs, ⌜@*xs =* ts⌝ ∧ A !> ≡ <! A[; *xs \ *ts ;] !>.
   Proof with auto.
     intros Hnodup Hfree. generalize dependent ts.
     induction xs as [|x xs' IH]; simpl in *; intros.
@@ -656,419 +654,381 @@ Section n_ary_lemmas.
   Lemma f_foralllist_one_point xs ts A `{OfSameLength _ _ xs ts} :
     NoDup xs →
     (list_to_set xs) ∩ ⋃ (term_fvars <$> ts) = ∅ →
-    <! ∀* xs, ⌜$(TVar <$> xs) =* ts⌝ ⇒ A !> ≡ <! A[; *xs \ *ts ;] !>.
+    <! ∀* xs, ⌜@*xs =* ts⌝ ⇒ A !> ≡ <! A[; *xs \ *ts ;] !>.
   Proof with auto.
     intros. rewrite f_foralllist_as_existslist. rewrite f_not_impl.
-    rewrite f_existslist_one_point.
-    - Unset Printing Notations.
-    intros Hnodup Hfree. generalize dependent ts.
-    induction xs as [|x xs' IH]; simpl in *; intros.
-    - inversion H. assert (H':=H). apply of_same_length_nil_inv_l in H' as ->.
-      simpl. unfold FEqList. simpl. rewrite f_true_implies...
-    - inversion H. assert (H':=H). apply of_same_length_cons_inv_l in H' as (t&ts'&?&?).
-      subst ts. rename ts' into ts. simpl. rewrite f_eqlist_cons.
-      apply NoDup_cons in Hnodup as []. rewrite <- IH by set_solver.
-      rewrite <- f_impl_curry. rewrite f_forall_list_impl_unused_l by set_solver.
-      rewrite f_forall_one_point by set_solver. f_equiv...
-  Qed.
-  Lemma f_exists_one_point x t A :
-      x ∉ term_fvars t →
-      <! ∃ x, ⌜x = t⌝ ∧ A !> ≡ <! A[x \ t] !>.
-  Proof with auto.
-    intros Hfree σ. simp feval. setoid_rewrite simpl_subst_and.
-    setoid_rewrite simpl_subst_af. simpl. destruct (decide (x = x)); [|contradiction].
-    clear e. split.
-    - intros [v Hv]. simp feval in Hv. destruct Hv as [H1 H2]. inversion H1.
-      destruct H as []. inversion H. subst v0 x0. clear H H1.
-      (* TODO: teval_subst looks ugly match it with feval_subst *)
-      rewrite <- (@teval_subst _ _ _ _ _ v _) in H0...
-      apply teval_delete_state_var_head in H0... rewrite (feval_subst v)...
-      rewrite <- (feval_subst _ (TConst v))...
-    - intros. pose proof (teval_total σ t) as [v Hv]. exists v. simp feval. split.
-      + simpl. exists v. split... rewrite <- (@teval_subst _ _ _ _ _ v _)...
-        rewrite teval_delete_state_var_head...
-      + rewrite (feval_subst v) in H... rewrite (feval_subst v)...
-  Qed.
-
-  (* A.56 *)
-  Lemma f_forall_one_point x t A :
-      x ∉ term_fvars t →
-      <! ∀ x, ⌜x = t⌝ ⇒ A !> ≡ <! A[x \ t] !>.
-  Proof with auto.
-    intros Hfree. unfold FForall. rewrite f_not_impl.
-    apply (f_exists_one_point x t(FNot A)) in Hfree. rewrite Hfree.
-    rewrite simpl_subst_not. rewrite f_not_stable...
+    rewrite f_existslist_one_point... rewrite simpl_seqsubst_not. rewrite f_not_stable...
   Qed.
 
   (* A.60 *)
-  Lemma f_exists_idemp x A :
-    <! ∃ x x, A !> ≡ <! ∃ x, A !>.
-  Proof with auto. rewrite fexists_unused... simpl. set_solver. Qed.
+  (* Lemma f_exists_idemp x A : *)
+  (*   <! ∃ x x, A !> ≡ <! ∃ x, A !>. *)
+  (* Proof with auto. rewrite fexists_unused... simpl. set_solver. Qed. *)
 
   (* A.59 *)
-  Lemma f_forall_idemp x A :
-    <! ∀ x x, A !> ≡ <! ∀ x, A !>.
-  Proof with auto. unfold FForall. rewrite f_not_stable. rewrite f_exists_idemp... Qed.
+  (* Lemma f_forall_idemp x A : *)
+  (*   <! ∀ x x, A !> ≡ <! ∀ x, A !>. *)
+  (* Proof with auto. unfold FForall. rewrite f_not_stable. rewrite f_exists_idemp... Qed. *)
 
 
   (* A.64 *)
-  Lemma f_exists_comm x y A :
-    <! ∃ x y, A !> ≡ <! ∃ y x, A !>.
-  Proof with auto.
-    intros σ. destruct (decide (x = y)). 1:{ subst... }
-    destruct (decide (x ∈ formula_fvars A)).
-    2:{ rewrite fexists_unused.
-        - rewrite (fexists_unused x)...
-        - simpl. set_solver. }
-    destruct (decide (y ∈ formula_fvars A)).
-    2:{ rewrite (fexists_unused y)...
-        rewrite (fexists_unused y)... simpl. set_solver. }
-    simp feval. split.
-    - intros [vx H]. rewrite (feval_subst vx) in H... simp feval in H. destruct H as [vy H].
-      rewrite (feval_subst vy) in H... exists vy. rewrite (feval_subst vy)...
-      simp feval. exists vx. rewrite (feval_subst vx)... rewrite (insert_commute σ)...
-    - intros [vy H]. rewrite (feval_subst vy) in H... simp feval in H. destruct H as [vx H].
-      rewrite (feval_subst vx) in H... exists vx. rewrite (feval_subst vx)...
-      simp feval. exists vy. rewrite (feval_subst vy)... rewrite (insert_commute σ)...
-  Qed.
+  (* Lemma f_exists_comm x y A : *)
+  (*   <! ∃ x y, A !> ≡ <! ∃ y x, A !>. *)
+  (* Proof with auto. *)
+  (*   intros σ. destruct (decide (x = y)). 1:{ subst... } *)
+  (*   destruct (decide (x ∈ formula_fvars A)). *)
+  (*   2:{ rewrite fexists_unused. *)
+  (*       - rewrite (fexists_unused x)... *)
+  (*       - simpl. set_solver. } *)
+  (*   destruct (decide (y ∈ formula_fvars A)). *)
+  (*   2:{ rewrite (fexists_unused y)... *)
+  (*       rewrite (fexists_unused y)... simpl. set_solver. } *)
+  (*   simp feval. split. *)
+  (*   - intros [vx H]. rewrite (feval_subst vx) in H... simp feval in H. destruct H as [vy H]. *)
+  (*     rewrite (feval_subst vy) in H... exists vy. rewrite (feval_subst vy)... *)
+  (*     simp feval. exists vx. rewrite (feval_subst vx)... rewrite (insert_commute σ)... *)
+  (*   - intros [vy H]. rewrite (feval_subst vy) in H... simp feval in H. destruct H as [vx H]. *)
+  (*     rewrite (feval_subst vx) in H... exists vx. rewrite (feval_subst vx)... *)
+  (*     simp feval. exists vy. rewrite (feval_subst vy)... rewrite (insert_commute σ)... *)
+  (* Qed. *)
 
   (* A.63 *)
-  Lemma f_forall_comm x y A :
-    <! ∀ x y, A !> ≡ <! ∀ y x, A !>.
-  Proof. unfold FForall. do 2 rewrite f_not_stable. rewrite f_exists_comm. reflexivity. Qed.
+  (* Lemma f_forall_comm x y A : *)
+  (*   <! ∀ x y, A !> ≡ <! ∀ y x, A !>. *)
+  (* Proof. unfold FForall. do 2 rewrite f_not_stable. rewrite f_exists_comm. reflexivity. Qed. *)
 
   (* A.66 *)
-  Lemma f_exists_or x A B :
-    <! ∃ x, A ∨ B !> ≡ <! (∃ x, A) ∨ (∃ x, B) !>.
-  Proof with auto.
-    intros σ. simp feval. setoid_rewrite simpl_subst_or. split.
-    - intros [v H]. simp feval in H. destruct H as [|]; [left|right]; exists v...
-    - intros [[v H] | [v H]]; exists v; simp feval...
-  Qed.
+  (* Lemma f_exists_or x A B : *)
+  (*   <! ∃ x, A ∨ B !> ≡ <! (∃ x, A) ∨ (∃ x, B) !>. *)
+  (* Proof with auto. *)
+  (*   intros σ. simp feval. setoid_rewrite simpl_subst_or. split. *)
+  (*   - intros [v H]. simp feval in H. destruct H as [|]; [left|right]; exists v... *)
+  (*   - intros [[v H] | [v H]]; exists v; simp feval... *)
+  (* Qed. *)
 
   (* A.65 *)
-  Lemma f_forall_and x A B :
-    <! ∀ x, A ∧ B !> ≡ <! (∀ x, A) ∧ (∀ x, B) !>.
-  Proof. unfold FForall. rewrite f_not_and. rewrite f_exists_or. rewrite f_not_or; auto. Qed.
+  (* Lemma f_forall_and x A B : *)
+  (*   <! ∀ x, A ∧ B !> ≡ <! (∀ x, A) ∧ (∀ x, B) !>. *)
+  (* Proof. unfold FForall. rewrite f_not_and. rewrite f_exists_or. rewrite f_not_or; auto. Qed. *)
 
   (* A.67 *)
-  Lemma f_exists_impl x A B :
-    <! ∃ x, A ⇒ B !> ≡ <! (∀ x, A) ⇒ (∃ x, B) !>.
-  Proof with auto.
-    intros σ. unfold FImpl. rewrite f_exists_or. unfold FForall. rewrite f_not_stable...
-  Qed.
+  (* Lemma f_exists_impl x A B : *)
+  (*   <! ∃ x, A ⇒ B !> ≡ <! (∀ x, A) ⇒ (∃ x, B) !>. *)
+  (* Proof with auto. *)
+  (*   intros σ. unfold FImpl. rewrite f_exists_or. unfold FForall. rewrite f_not_stable... *)
+  (* Qed. *)
 
   (* A.68 *)
-  Lemma f_forall_ent_exists x A :
-    <! ∀ x, A !> ⇛ <! ∃ x, A !>.
-  Proof.
-    intros σ. rewrite simpl_feval_fforall. intros. simp feval.
-    exists ⊥. apply H.
-  Qed.
+  (* Lemma f_forall_ent_exists x A : *)
+  (*   <! ∀ x, A !> ⇛ <! ∃ x, A !>. *)
+  (* Proof. *)
+  (*   intros σ. rewrite simpl_feval_fforall. intros. simp feval. *)
+  (*   exists ⊥. apply H. *)
+  (* Qed. *)
 
   (* A.69 *)
-  Lemma f_or_forall x A B :
-    <! (∀ x, A) ∨ (∀ x, B) !> ⇛ <! ∀ x, A ∨ B !>.
-  Proof.
-    intros σ. simp feval. do 3 rewrite simpl_feval_fforall.
-    setoid_rewrite simpl_subst_or.
-    intros [|]; intros; simp feval; naive_solver.
-  Qed.
+  (* Lemma f_or_forall x A B : *)
+  (*   <! (∀ x, A) ∨ (∀ x, B) !> ⇛ <! ∀ x, A ∨ B !>. *)
+  (* Proof. *)
+  (*   intros σ. simp feval. do 3 rewrite simpl_feval_fforall. *)
+  (*   setoid_rewrite simpl_subst_or. *)
+  (*   intros [|]; intros; simp feval; naive_solver. *)
+  (* Qed. *)
 
   (* A.70 *)
-  Lemma f_forall_impl x A B :
-    <! ∀ x, A ⇒ B !> ⇛ <! (∀ x, A) ⇒ (∀ x, B) !>.
-  Proof.
-    intros σ. rewrite simpl_feval_fimpl. do 3 rewrite simpl_feval_fforall.
-    intros. specialize (H v). rewrite simpl_subst_impl in H. rewrite simpl_feval_fimpl in H.
-    naive_solver.
-  Qed.
+  (* Lemma f_forall_impl x A B : *)
+  (*   <! ∀ x, A ⇒ B !> ⇛ <! (∀ x, A) ⇒ (∀ x, B) !>. *)
+  (* Proof. *)
+  (*   intros σ. rewrite simpl_feval_fimpl. do 3 rewrite simpl_feval_fforall. *)
+  (*   intros. specialize (H v). rewrite simpl_subst_impl in H. rewrite simpl_feval_fimpl in H. *)
+  (*   naive_solver. *)
+  (* Qed. *)
 
   (* A.71 *)
-  Lemma f_exists_and x A B :
-    <! ∃ x, A ∧ B !> ⇛ <! (∃ x, A) ∧ (∃ x, B) !>.
-  Proof with auto.
-    intros σ. simp feval. intros [v H]. rewrite simpl_subst_and in H. simp feval in H.
-    destruct H as []. split; exists v...
-  Qed.
+  (* Lemma f_exists_and x A B : *)
+  (*   <! ∃ x, A ∧ B !> ⇛ <! (∃ x, A) ∧ (∃ x, B) !>. *)
+  (* Proof with auto. *)
+  (*   intros σ. simp feval. intros [v H]. rewrite simpl_subst_and in H. simp feval in H. *)
+  (*   destruct H as []. split; exists v... *)
+  (* Qed. *)
 
   (* A.72 *)
-  Lemma f_impl_exists x A B :
-    <! (∃ x, A) ⇒ (∃ x, B) !> ⇛ <! ∃ x, A ⇒ B !>.
-  Proof with auto.
-    intros σ. rewrite simpl_feval_fimpl. intros. simp feval.
-    setoid_rewrite simpl_subst_impl. setoid_rewrite simpl_feval_fimpl.
-    destruct (feval_lem σ <! ∃ x, A !>).
-    - apply H in H0. simp feval in H0. destruct H0 as [v Hv]. exists v. intros...
-    - exists ⊥. intros. simp feval in H0. exfalso. apply H0. exists ⊥...
-  Qed.
+  (* Lemma f_impl_exists x A B : *)
+  (*   <! (∃ x, A) ⇒ (∃ x, B) !> ⇛ <! ∃ x, A ⇒ B !>. *)
+  (* Proof with auto. *)
+  (*   intros σ. rewrite simpl_feval_fimpl. intros. simp feval. *)
+  (*   setoid_rewrite simpl_subst_impl. setoid_rewrite simpl_feval_fimpl. *)
+  (*   destruct (feval_lem σ <! ∃ x, A !>). *)
+  (*   - apply H in H0. simp feval in H0. destruct H0 as [v Hv]. exists v. intros... *)
+  (*   - exists ⊥. intros. simp feval in H0. exfalso. apply H0. exists ⊥... *)
+  (* Qed. *)
 
   (* A.73 *)
-  Lemma f_exists_forall x y A :
-    <! ∃ x, (∀ y, A) !> ⇛ <! ∀ y, (∃ x, A) !>.
-  Proof with auto.
-    intros σ. simp feval. rewrite simpl_feval_fforall. intros [vx H] vy.
-    destruct (decide (x = y)).
-    1:{ subst y. rewrite simpl_subst_forall_skip in H... rewrite simpl_subst_exists_skip...
-        apply f_forall_ent_exists in H... }
-    rewrite (feval_subst vx) in H... rewrite simpl_feval_fforall in H.
-    specialize (H vy). rewrite (feval_subst vy) in H...
-    rewrite (feval_subst vy)... simp feval. exists vx. rewrite (feval_subst vx)...
-    rewrite (insert_commute σ)...
-  Qed.
+  (* Lemma f_exists_forall x y A : *)
+  (*   <! ∃ x, (∀ y, A) !> ⇛ <! ∀ y, (∃ x, A) !>. *)
+  (* Proof with auto. *)
+  (*   intros σ. simp feval. rewrite simpl_feval_fforall. intros [vx H] vy. *)
+  (*   destruct (decide (x = y)). *)
+  (*   1:{ subst y. rewrite simpl_subst_forall_skip in H... rewrite simpl_subst_exists_skip... *)
+  (*       apply f_forall_ent_exists in H... } *)
+  (*   rewrite (feval_subst vx) in H... rewrite simpl_feval_fforall in H. *)
+  (*   specialize (H vy). rewrite (feval_subst vy) in H... *)
+  (*   rewrite (feval_subst vy)... simp feval. exists vx. rewrite (feval_subst vx)... *)
+  (*   rewrite (insert_commute σ)... *)
+  (* Qed. *)
 
   (* A.74: fforall_unused *)
   (* A.75: fexists_unused *)
 
   (* A.76 *)
-  Lemma f_forall_and_unused_l x A B :
-    x ∉ formula_fvars A →
-    <! ∀ x, A ∧ B !> ≡ <! A ∧ (∀ x, B) !>.
-  Proof with auto. intros. rewrite f_forall_and. rewrite fforall_unused... Qed.
+  (* Lemma f_forall_and_unused_l x A B : *)
+  (*   x ∉ formula_fvars A → *)
+  (*   <! ∀ x, A ∧ B !> ≡ <! A ∧ (∀ x, B) !>. *)
+  (* Proof with auto. intros. rewrite f_forall_and. rewrite fforall_unused... Qed. *)
 
   (* A.76' *)
-  Lemma f_forall_and_unused_r x A B :
-    x ∉ formula_fvars B →
-    <! ∀ x, A ∧ B !> ≡ <! (∀ x, A) ∧ B !>.
-  Proof with auto. intros. rewrite f_forall_and. rewrite (fforall_unused x B)... Qed.
+  (* Lemma f_forall_and_unused_r x A B : *)
+  (*   x ∉ formula_fvars B → *)
+  (*   <! ∀ x, A ∧ B !> ≡ <! (∀ x, A) ∧ B !>. *)
+  (* Proof with auto. intros. rewrite f_forall_and. rewrite (fforall_unused x B)... Qed. *)
 
   (* A.77 *)
-  Lemma f_forall_or_unused_l x A B :
-    x ∉ formula_fvars A →
-    <! ∀ x, A ∨ B !> ≡ <! A ∨ (∀ x, B) !>.
-  Proof with auto.
-    intros. intros σ. rewrite simpl_feval_fforall. setoid_rewrite simpl_subst_or.
-    split; intros.
-    - simp feval. destruct (feval_lem σ A)... right. rewrite simpl_feval_fforall.
-      intros. specialize (H0 v). simp feval in H0. destruct H0...
-      rewrite (feval_subst v) in H0... apply feval_delete_state_var_head in H0...
-      contradiction.
-    - simp feval in *. rewrite (feval_subst v)... rewrite feval_delete_state_var_head...
-      destruct H0... right. rewrite simpl_feval_fforall in H0. apply H0.
-  Qed.
+  (* Lemma f_forall_or_unused_l x A B : *)
+  (*   x ∉ formula_fvars A → *)
+  (*   <! ∀ x, A ∨ B !> ≡ <! A ∨ (∀ x, B) !>. *)
+  (* Proof with auto. *)
+  (*   intros. intros σ. rewrite simpl_feval_fforall. setoid_rewrite simpl_subst_or. *)
+  (*   split; intros. *)
+  (*   - simp feval. destruct (feval_lem σ A)... right. rewrite simpl_feval_fforall. *)
+  (*     intros. specialize (H0 v). simp feval in H0. destruct H0... *)
+  (*     rewrite (feval_subst v) in H0... apply feval_delete_state_var_head in H0... *)
+  (*     contradiction. *)
+  (*   - simp feval in *. rewrite (feval_subst v)... rewrite feval_delete_state_var_head... *)
+  (*     destruct H0... right. rewrite simpl_feval_fforall in H0. apply H0. *)
+  (* Qed. *)
 
   (* A.77' *)
-  Lemma f_forall_or_unused_r x A B :
-    x ∉ formula_fvars B →
-    <! ∀ x, A ∨ B !> ≡ <! (∀ x, A) ∨ B !>.
-  Proof with auto.
-    intros. intros σ. rewrite simpl_feval_fforall. setoid_rewrite simpl_subst_or.
-    split; intros.
-    - simp feval. destruct (feval_lem σ B)... left. rewrite simpl_feval_fforall.
-      intros. specialize (H0 v). simp feval in H0. destruct H0...
-      rewrite (feval_subst v) in H0... apply feval_delete_state_var_head in H0...
-      contradiction.
-    - simp feval in *. destruct H0.
-      + left. rewrite simpl_feval_fforall in H0. apply H0...
-      + right. rewrite (feval_subst v)... rewrite feval_delete_state_var_head...
-  Qed.
+  (* Lemma f_forall_or_unused_r x A B : *)
+  (*   x ∉ formula_fvars B → *)
+  (*   <! ∀ x, A ∨ B !> ≡ <! (∀ x, A) ∨ B !>. *)
+  (* Proof with auto. *)
+  (*   intros. intros σ. rewrite simpl_feval_fforall. setoid_rewrite simpl_subst_or. *)
+  (*   split; intros. *)
+  (*   - simp feval. destruct (feval_lem σ B)... left. rewrite simpl_feval_fforall. *)
+  (*     intros. specialize (H0 v). simp feval in H0. destruct H0... *)
+  (*     rewrite (feval_subst v) in H0... apply feval_delete_state_var_head in H0... *)
+  (*     contradiction. *)
+  (*   - simp feval in *. destruct H0. *)
+  (*     + left. rewrite simpl_feval_fforall in H0. apply H0... *)
+  (*     + right. rewrite (feval_subst v)... rewrite feval_delete_state_var_head... *)
+  (* Qed. *)
 
   (* A.78 *)
-  Lemma f_forall_impl_unused_l x A B :
-    x ∉ formula_fvars A →
-    <! ∀ x, A ⇒ B !> ≡ <! A ⇒ (∀ x, B) !>.
-  Proof with auto.
-    intros. intros σ. rewrite simpl_feval_fforall. setoid_rewrite simpl_subst_impl.
-    rewrite simpl_feval_fimpl.
-    split; intros.
-    - rewrite simpl_feval_fforall. intros. specialize (H0 v). rewrite simpl_feval_fimpl in H0.
-      rewrite (feval_subst v) in H0... rewrite feval_delete_state_var_head in H0...
-    - rewrite simpl_feval_fimpl. intros. rewrite (feval_subst v) in H1...
-      rewrite feval_delete_state_var_head in H1... apply H0 in H1.
-      rewrite simpl_feval_fforall in H1...
-  Qed.
+  (* Lemma f_forall_impl_unused_l x A B : *)
+  (*   x ∉ formula_fvars A → *)
+  (*   <! ∀ x, A ⇒ B !> ≡ <! A ⇒ (∀ x, B) !>. *)
+  (* Proof with auto. *)
+  (*   intros. intros σ. rewrite simpl_feval_fforall. setoid_rewrite simpl_subst_impl. *)
+  (*   rewrite simpl_feval_fimpl. *)
+  (*   split; intros. *)
+  (*   - rewrite simpl_feval_fforall. intros. specialize (H0 v). rewrite simpl_feval_fimpl in H0. *)
+  (*     rewrite (feval_subst v) in H0... rewrite feval_delete_state_var_head in H0... *)
+  (*   - rewrite simpl_feval_fimpl. intros. rewrite (feval_subst v) in H1... *)
+  (*     rewrite feval_delete_state_var_head in H1... apply H0 in H1. *)
+  (*     rewrite simpl_feval_fforall in H1... *)
+  (* Qed. *)
 
   (* A.79 *)
-  Lemma f_forall_impl_unused_r x A B :
-    x ∉ formula_fvars B →
-    <! ∀ x, A ⇒ B !> ≡ <! (∃ x, A) ⇒ B !>.
-  Proof with auto.
-    intros. intros σ. rewrite simpl_feval_fforall. setoid_rewrite simpl_subst_impl.
-    setoid_rewrite simpl_feval_fimpl. simp feval.
-    split; intros.
-    - destruct H1 as [v Hv]. apply H0 in Hv. apply (feval_subst v) in Hv...
-      apply feval_delete_state_var_head in Hv...
-    - forward H0 by (exists v)... apply (feval_subst v)... apply feval_delete_state_var_head...
-  Qed.
+  (* Lemma f_forall_impl_unused_r x A B : *)
+  (*   x ∉ formula_fvars B → *)
+  (*   <! ∀ x, A ⇒ B !> ≡ <! (∃ x, A) ⇒ B !>. *)
+  (* Proof with auto. *)
+  (*   intros. intros σ. rewrite simpl_feval_fforall. setoid_rewrite simpl_subst_impl. *)
+  (*   setoid_rewrite simpl_feval_fimpl. simp feval. *)
+  (*   split; intros. *)
+  (*   - destruct H1 as [v Hv]. apply H0 in Hv. apply (feval_subst v) in Hv... *)
+  (*     apply feval_delete_state_var_head in Hv... *)
+  (*   - forward H0 by (exists v)... apply (feval_subst v)... apply feval_delete_state_var_head... *)
+  (* Qed. *)
 
   (* A.80 *)
-  Lemma f_exists_and_unused_l x A B :
-    x ∉ formula_fvars A →
-    <! ∃ x, A ∧ B !> ≡ <! A ∧ (∃ x, B) !>.
-  Proof with auto.
-    intros. rewrite <- (f_not_stable A). rewrite <- (f_not_stable B). rewrite <- (f_not_or).
-    rewrite <- (f_not_forall). rewrite f_forall_or_unused_l by (simpl; auto).
-    rewrite f_not_or. rewrite f_not_forall...
-  Qed.
+  (* Lemma f_exists_and_unused_l x A B : *)
+  (*   x ∉ formula_fvars A → *)
+  (*   <! ∃ x, A ∧ B !> ≡ <! A ∧ (∃ x, B) !>. *)
+  (* Proof with auto. *)
+  (*   intros. rewrite <- (f_not_stable A). rewrite <- (f_not_stable B). rewrite <- (f_not_or). *)
+  (*   rewrite <- (f_not_forall). rewrite f_forall_or_unused_l by (simpl; auto). *)
+  (*   rewrite f_not_or. rewrite f_not_forall... *)
+  (* Qed. *)
 
   (* A.80' *)
-  Lemma f_exists_and_unused_r x A B :
-    x ∉ formula_fvars B →
-    <! ∃ x, A ∧ B !> ≡ <! (∃ x, A) ∧ B !>.
-  Proof with auto.
-    intros. rewrite <- (f_not_stable A). rewrite <- (f_not_stable B). rewrite <- (f_not_or).
-    rewrite <- (f_not_forall). rewrite f_forall_or_unused_r by (simpl; auto).
-    rewrite f_not_or. rewrite f_not_forall...
-  Qed.
+  (* Lemma f_exists_and_unused_r x A B : *)
+  (*   x ∉ formula_fvars B → *)
+  (*   <! ∃ x, A ∧ B !> ≡ <! (∃ x, A) ∧ B !>. *)
+  (* Proof with auto. *)
+  (*   intros. rewrite <- (f_not_stable A). rewrite <- (f_not_stable B). rewrite <- (f_not_or). *)
+  (*   rewrite <- (f_not_forall). rewrite f_forall_or_unused_r by (simpl; auto). *)
+  (*   rewrite f_not_or. rewrite f_not_forall... *)
+  (* Qed. *)
 
   (* A.81 *)
-  Lemma f_exists_or_unused_l x A B :
-    x ∉ formula_fvars A →
-    <! ∃ x, A ∨ B !> ≡ <! A ∨ (∃ x, B) !>.
-  Proof with auto. intros. rewrite f_exists_or. rewrite fexists_unused... Qed.
+  (* Lemma f_exists_or_unused_l x A B : *)
+  (*   x ∉ formula_fvars A → *)
+  (*   <! ∃ x, A ∨ B !> ≡ <! A ∨ (∃ x, B) !>. *)
+  (* Proof with auto. intros. rewrite f_exists_or. rewrite fexists_unused... Qed. *)
 
   (* A.81' *)
-  Lemma f_exists_or_unused_r x A B :
-    x ∉ formula_fvars B →
-    <! ∃ x, A ∨ B !> ≡ <! (∃ x, A) ∨ B !>.
-  Proof with auto. intros. rewrite f_exists_or. rewrite (fexists_unused _ B)... Qed.
+  (* Lemma f_exists_or_unused_r x A B : *)
+  (*   x ∉ formula_fvars B → *)
+  (*   <! ∃ x, A ∨ B !> ≡ <! (∃ x, A) ∨ B !>. *)
+  (* Proof with auto. intros. rewrite f_exists_or. rewrite (fexists_unused _ B)... Qed. *)
 
   (* A.82 *)
-  Lemma f_exists_impl_unused_l x A B :
-    x ∉ formula_fvars A →
-    <! ∃ x, A ⇒ B !> ≡ <! A ⇒ (∃ x, B) !>.
-  Proof with auto. intros. rewrite f_exists_impl. rewrite fforall_unused... Qed.
+  (* Lemma f_exists_impl_unused_l x A B : *)
+  (*   x ∉ formula_fvars A → *)
+  (*   <! ∃ x, A ⇒ B !> ≡ <! A ⇒ (∃ x, B) !>. *)
+  (* Proof with auto. intros. rewrite f_exists_impl. rewrite fforall_unused... Qed. *)
 
   (* A.83 *)
-  Lemma f_exists_impl_unused_r x A B :
-    x ∉ formula_fvars B →
-    <! ∃ x, A ⇒ B !> ≡ <! (∀ x, A) ⇒ B !>.
-  Proof with auto. intros. rewrite f_exists_impl. rewrite fexists_unused... Qed.
+  (* Lemma f_exists_impl_unused_r x A B : *)
+  (*   x ∉ formula_fvars B → *)
+  (*   <! ∃ x, A ⇒ B !> ≡ <! (∀ x, A) ⇒ B !>. *)
+  (* Proof with auto. intros. rewrite f_exists_impl. rewrite fexists_unused... Qed. *)
 
   (* A.84: fforall_alpha_equiv *)
   (* A.85: fexists_alpha_equiv *)
 
   (* A.86 *)
-  Lemma f_forall_elim t x A :
-    <! ∀ x, A !> ⇛ <! A[x \ t] !>.
-  Proof with auto.
-    intros σ. rewrite simpl_feval_fforall. intros. pose proof (teval_total σ t) as [v Hv].
-    specialize (H v). rewrite (feval_subst v) in H... rewrite (feval_subst v)...
-  Qed.
+  (* Lemma f_forall_elim t x A : *)
+  (*   <! ∀ x, A !> ⇛ <! A[x \ t] !>. *)
+  (* Proof with auto. *)
+  (*   intros σ. rewrite simpl_feval_fforall. intros. pose proof (teval_total σ t) as [v Hv]. *)
+  (*   specialize (H v). rewrite (feval_subst v) in H... rewrite (feval_subst v)... *)
+  (* Qed. *)
 
   (* A.86 *)
-  Lemma f_exists_intro t x A :
-    <! A[x \ t] !> ⇛ <! ∃ x, A !>.
-  Proof with auto.
-    intros σ. simp feval. intros. pose proof (teval_total σ t) as [v Hv].
-    exists v. rewrite (feval_subst v) in H... rewrite (feval_subst v)...
-  Qed.
+  (* Lemma f_exists_intro t x A : *)
+  (*   <! A[x \ t] !> ⇛ <! ∃ x, A !>. *)
+  (* Proof with auto. *)
+  (*   intros σ. simp feval. intros. pose proof (teval_total σ t) as [v Hv]. *)
+  (*   exists v. rewrite (feval_subst v) in H... rewrite (feval_subst v)... *)
+  (* Qed. *)
 
-  Lemma f_impl_elim A B :
-    <! A ∧ (A ⇒ B) !> ⇛ B.
-  Proof with auto.
-    intros σ. simp feval. rewrite simpl_feval_fimpl. naive_solver.
-  Qed.
+  (* Lemma f_impl_elim A B : *)
+  (*   <! A ∧ (A ⇒ B) !> ⇛ B. *)
+  (* Proof with auto. *)
+  (*   intros σ. simp feval. rewrite simpl_feval_fimpl. naive_solver. *)
+  (* Qed. *)
 
   (* some lemmas for proving equivalences and entailments *)
 
-  Lemma f_and_cancel_l A B C :
-    B ≡ C → <! A ∧ B !> ≡ <! A ∧ C !>.
-  Proof. intros. rewrite H. reflexivity. Qed.
+  (* Lemma f_and_cancel_l A B C : *)
+  (*   B ≡ C → <! A ∧ B !> ≡ <! A ∧ C !>. *)
+  (* Proof. intros. rewrite H. reflexivity. Qed. *)
 
-  Lemma f_and_cancel_r A B C :
-    B ≡ C → <! B ∧ A !> ≡ <! C ∧ A !>.
-  Proof. intros. rewrite H. reflexivity. Qed.
+  (* Lemma f_and_cancel_r A B C : *)
+  (*   B ≡ C → <! B ∧ A !> ≡ <! C ∧ A !>. *)
+  (* Proof. intros. rewrite H. reflexivity. Qed. *)
 
-  Lemma f_or_cancel_l A B C :
-    B ≡ C → <! A ∨ B !> ≡ <! A ∨ C !>.
-  Proof. intros. rewrite H. reflexivity. Qed.
+  (* Lemma f_or_cancel_l A B C : *)
+  (*   B ≡ C → <! A ∨ B !> ≡ <! A ∨ C !>. *)
+  (* Proof. intros. rewrite H. reflexivity. Qed. *)
 
-  Lemma f_or_cancel_r A B C :
-    B ≡ C → <! B ∨ A !> ≡ <! C ∨ A !>.
-  Proof. intros. rewrite H. reflexivity. Qed.
+  (* Lemma f_or_cancel_r A B C : *)
+  (*   B ≡ C → <! B ∨ A !> ≡ <! C ∨ A !>. *)
+  (* Proof. intros. rewrite H. reflexivity. Qed. *)
 
-  Lemma f_impl_cancel_l A B C :
-    B ≡ C → <! A ⇒ B !> ≡ <! A ⇒ C !>.
-  Proof. intros. rewrite H. reflexivity. Qed.
+  (* Lemma f_impl_cancel_l A B C : *)
+  (*   B ≡ C → <! A ⇒ B !> ≡ <! A ⇒ C !>. *)
+  (* Proof. intros. rewrite H. reflexivity. Qed. *)
 
-  Lemma f_impl_cancel_r A B C :
-    B ≡ C → <! B ⇒ A !> ≡ <! C ⇒ A !>.
-  Proof. intros. rewrite H. reflexivity. Qed.
+  (* Lemma f_impl_cancel_r A B C : *)
+  (*   B ≡ C → <! B ⇒ A !> ≡ <! C ⇒ A !>. *)
+  (* Proof. intros. rewrite H. reflexivity. Qed. *)
 
-  Lemma f_subst_cancel A B x t :
-    A ≡ B → <! A[x \ t] !> ≡ <! B[x \ t] !>.
-  Proof. intros. rewrite H. reflexivity. Qed.
+  (* Lemma f_subst_cancel A B x t : *)
+  (*   A ≡ B → <! A[x \ t] !> ≡ <! B[x \ t] !>. *)
+  (* Proof. intros. rewrite H. reflexivity. Qed. *)
 
-  Lemma f_subst_cancel_term A x t1 t2 :
-    t1 ≡ t2 → <! A[x \ t1] !> ≡ <! A[x \ t2] !>.
-  Proof. intros. rewrite H. reflexivity. Qed.
+  (* Lemma f_subst_cancel_term A x t1 t2 : *)
+  (*   t1 ≡ t2 → <! A[x \ t1] !> ≡ <! A[x \ t2] !>. *)
+  (* Proof. intros. rewrite H. reflexivity. Qed. *)
 
-  Lemma f_exists_equiv A B y1 y2 :
-    (∀ t, <! A[y1 \ t] !> ≡ <! B[y2 \ t] !>) →
-    <! ∃ y1, A !> ≡ <! ∃ y2, B !>.
-  Proof. intros Hequiv σ. apply feval_exists_equiv_if. naive_solver. Qed.
+  (* Lemma f_exists_equiv A B y1 y2 : *)
+  (*   (∀ t, <! A[y1 \ t] !> ≡ <! B[y2 \ t] !>) → *)
+  (*   <! ∃ y1, A !> ≡ <! ∃ y2, B !>. *)
+  (* Proof. intros Hequiv σ. apply feval_exists_equiv_if. naive_solver. Qed. *)
 
-  Lemma f_forall_equiv A B y1 y2 :
-    (∀ t, <! A[y1 \ t] !> ≡ <! B[y2 \ t] !>) →
-    <! ∀ y1, A !> ≡ <! ∀ y2, B !>.
-  Proof. intros Hequiv σ. do 2 rewrite simpl_feval_fforall. naive_solver. Qed.
+  (* Lemma f_forall_equiv A B y1 y2 : *)
+  (*   (∀ t, <! A[y1 \ t] !> ≡ <! B[y2 \ t] !>) → *)
+  (*   <! ∀ y1, A !> ≡ <! ∀ y2, B !>. *)
+  (* Proof. intros Hequiv σ. do 2 rewrite simpl_feval_fforall. naive_solver. Qed. *)
 
-  Lemma f_ent_and_cancel_l A B C :
-    B ⇛ C → <! A ∧ B !> ⇛ <! A ∧ C !>.
-  Proof. intros H σ. simp feval. specialize (H σ). naive_solver. Qed.
+  (* Lemma f_ent_and_cancel_l A B C : *)
+  (*   B ⇛ C → <! A ∧ B !> ⇛ <! A ∧ C !>. *)
+  (* Proof. intros H σ. simp feval. specialize (H σ). naive_solver. Qed. *)
 
-  Lemma f_ent_and_cancel_r A B C :
-    B ⇛ C → <! B ∧ A !> ⇛ <! C ∧ A !>.
-  Proof. intros H σ. simp feval. specialize (H σ). naive_solver. Qed.
+  (* Lemma f_ent_and_cancel_r A B C : *)
+  (*   B ⇛ C → <! B ∧ A !> ⇛ <! C ∧ A !>. *)
+  (* Proof. intros H σ. simp feval. specialize (H σ). naive_solver. Qed. *)
 
-  Lemma f_ent_or_cancel_l A B C :
-    B ⇛ C → <! A ∨ B !> ⇛ <! A ∨ C !>.
-  Proof. intros H σ. simp feval. specialize (H σ). naive_solver. Qed.
+  (* Lemma f_ent_or_cancel_l A B C : *)
+  (*   B ⇛ C → <! A ∨ B !> ⇛ <! A ∨ C !>. *)
+  (* Proof. intros H σ. simp feval. specialize (H σ). naive_solver. Qed. *)
 
-  Lemma f_ent_or_cancel_r A B C :
-    B ⇛ C → <! B ∨ A !> ⇛ <! C ∨ A !>.
-  Proof. intros H σ. simp feval. specialize (H σ). naive_solver. Qed.
+  (* Lemma f_ent_or_cancel_r A B C : *)
+  (*   B ⇛ C → <! B ∨ A !> ⇛ <! C ∨ A !>. *)
+  (* Proof. intros H σ. simp feval. specialize (H σ). naive_solver. Qed. *)
 
-  Lemma f_ent_subst_cancel A B x t :
-    A ⇛ B → <! A[x \ t] !> ⇛ <! B[x \ t] !>.
-  Proof with auto.
-    intros Hent σ H. pose proof (teval_total σ t) as [v Hv]. rewrite (feval_subst v) in H...
-    apply Hent in H. rewrite (feval_subst v)...
-  Qed.
+  (* Lemma f_ent_subst_cancel A B x t : *)
+  (*   A ⇛ B → <! A[x \ t] !> ⇛ <! B[x \ t] !>. *)
+  (* Proof with auto. *)
+  (*   intros Hent σ H. pose proof (teval_total σ t) as [v Hv]. rewrite (feval_subst v) in H... *)
+  (*   apply Hent in H. rewrite (feval_subst v)... *)
+  (* Qed. *)
 
-  Lemma f_ent_impl_cancel_l A B C :
-    B ⇛ C → <! A ⇒ B !> ⇛ <! A ⇒ C !>.
-  Proof. intros H σ. do 2 rewrite simpl_feval_fimpl. naive_solver. Qed.
+  (* Lemma f_ent_impl_cancel_l A B C : *)
+  (*   B ⇛ C → <! A ⇒ B !> ⇛ <! A ⇒ C !>. *)
+  (* Proof. intros H σ. do 2 rewrite simpl_feval_fimpl. naive_solver. Qed. *)
 
-  Lemma f_ent_impl_cancel_r A B C :
-    C ⇛ B → <! B ⇒ A !> ⇛ <! C ⇒ A !>.
-  Proof. intros H σ. do 2 rewrite simpl_feval_fimpl. naive_solver. Qed.
+  (* Lemma f_ent_impl_cancel_r A B C : *)
+  (*   C ⇛ B → <! B ⇒ A !> ⇛ <! C ⇒ A !>. *)
+  (* Proof. intros H σ. do 2 rewrite simpl_feval_fimpl. naive_solver. Qed. *)
 
-  Lemma f_exists_ent A B y1 y2 :
-    (∀ t, <! A[y1 \ t] !> ⇛ <! B[y2 \ t] !>) →
-    <! ∃ y1, A !> ⇛ <! ∃ y2, B !>.
-  Proof.
-    intros Hequiv σ. simp feval. intros [v Hv]. exists v. naive_solver.
-  Qed.
+  (* Lemma f_exists_ent A B y1 y2 : *)
+  (*   (∀ t, <! A[y1 \ t] !> ⇛ <! B[y2 \ t] !>) → *)
+  (*   <! ∃ y1, A !> ⇛ <! ∃ y2, B !>. *)
+  (* Proof. *)
+  (*   intros Hequiv σ. simp feval. intros [v Hv]. exists v. naive_solver. *)
+  (* Qed. *)
 
-  Lemma f_forall_ent A B y1 y2 :
-    (∀ t, <! A[y1 \ t] !> ⇛ <! B[y2 \ t] !>) →
-    <! ∀ y1, A !> ⇛ <! ∀ y2, B !>.
-  Proof.
-    intros Hequiv σ. do 2 rewrite simpl_feval_fforall. intros. naive_solver.
-  Qed.
+  (* Lemma f_forall_ent A B y1 y2 : *)
+  (*   (∀ t, <! A[y1 \ t] !> ⇛ <! B[y2 \ t] !>) → *)
+  (*   <! ∀ y1, A !> ⇛ <! ∀ y2, B !>. *)
+  (* Proof. *)
+  (*   intros Hequiv σ. do 2 rewrite simpl_feval_fforall. intros. naive_solver. *)
+  (* Qed. *)
 
-  Lemma f_ent_elim σ A B :
-    feval σ A →
-    A ⇛ B →
-    feval σ B.
-  Proof. naive_solver. Qed.
+  (* Lemma f_ent_elim σ A B : *)
+  (*   feval σ A → *)
+  (*   A ⇛ B → *)
+  (*   feval σ B. *)
+  (* Proof. naive_solver. Qed. *)
 
-  Lemma f_ent_intro A B :
-    (∀ σ, feval σ A → feval σ B) →
-    A ⇛ B.
-  Proof. naive_solver. Qed.
+  (* Lemma f_ent_intro A B : *)
+  (*   (∀ σ, feval σ A → feval σ B) → *)
+  (*   A ⇛ B. *)
+  (* Proof. naive_solver. Qed. *)
 
-  Lemma f_eq_refl t :
-    <! ⌜t = t⌝ !> ≡ <! true !>.
-  Proof.
-    prove_equiv. intros. destruct (teval_total σ t) as [v Hv]. econstructor. split; exact Hv.
-  Qed.
+  (* Lemma f_eq_refl t : *)
+  (*   <! ⌜t = t⌝ !> ≡ <! true !>. *)
+  (* Proof. *)
+  (*   prove_equiv. intros. destruct (teval_total σ t) as [v Hv]. econstructor. split; exact Hv. *)
+  (* Qed. *)
 
-  Lemma f_neq_irrefl t :
-    <! ⌜t ≠ t⌝ !> ≡ <! false !>.
-  Proof.
-    rewrite f_eq_refl. rewrite f_not_true. reflexivity.
-  Qed.
+  (* Lemma f_neq_irrefl t : *)
+  (*   <! ⌜t ≠ t⌝ !> ≡ <! false !>. *)
+  (* Proof. *)
+  (*   rewrite f_eq_refl. rewrite f_not_true. reflexivity. *)
+  (* Qed. *)
 End n_ary_lemmas.
